\begin{array}{cc}
\mathrm{Quadratic\ Equation} & {x}=\frac{-{b}\pm \sqrt{{{b}}_{}^{2}-4{a}{c}}}{2{a}}  \\
\mathrm{DisplayQuadratic\ Equation} & {x}=\frac{-{b}\pm \sqrt{{{b}}_{}^{2}-4{a}{c}}}{2{a}}  \\
\mathrm{Rational\ Function} & {f}({x})=\frac{1-{{x}}_{}^{2}}{1-{{x}}_{}^{3}}  \\
\mathrm{Rational\ Function} & {f}({x})=\frac{(1-{{x}}_{}^{2}){{x}}_{}^{3}}{1-{{x}}_{}^{3}}  \\
\mathrm{Rational\ Function} & {f}({x})=\frac{(1-{{x}}_{}^{2})({{x}}_{}^{3}-5{x})}{1-{{x}}_{}^{3}}  \\
\mathrm{Parametrize\ Rational\ Function} & {f}({x})=\frac{({{a}}_{{i}}^{}-{{x}}_{}^{2}{)}_{}^{5}}{1-{{x}}_{}^{3}}  \\
\mathrm{Stacked\ exponents} & {g}({z})={{e}}_{}^{-{{x}}_{}^{2}} \\
\mathrm{Stacked\ exponents} & {g}({z})={{e}}_{}^{-({z}-{a}{)}_{}^{2}} \\
\mathrm{Stacked\ exponents} & {g}({z})={{e}}_{}^{-\underset{{i}=0}{\overset{{\infty }}{\sum }}{{z}}_{{i}}^{2}} \\
\mathrm{Stacked\ exponents} & {g}({y})={{e}}_{}^{-\underset{{i}=0}{\overset{{\infty }}{\sum }}{{y}}_{{i}}^{2}} \\
\mathrm{Stacked\ exponents} & {g}({z})={{e}}_{}^{-\underset{{i}=0}{\overset{{\infty }}{\sum }}{{z}}_{}^{\frac{2}{{a}-{i}} }} \\
\mathrm{Cross\ Product} & \frac{{{x}}_{1}^{}-{{x}}_{2}^{}}{{{x}}_{3}^{}-{{x}}_{4}^{}} \frac{{{x}}_{1}^{}-{{x}}_{4}^{}}{{{x}}_{2}^{}-{{x}}_{3}^{}}  \\
\mathrm{Cross\ Product} & (\frac{{{x}}_{1}^{}-{{x}}_{2}^{}}{{{x}}_{3}^{}-{{x}}_{4}^{}} )(\frac{{{x}}_{1}^{}-{{x}}_{4}^{}}{{{x}}_{2}^{}-{{x}}_{3}^{}} ) \\
\mathrm{Cross\ Product} & \left( \frac{{{x}}_{1}^{}-{{x}}_{2}^{}}{{{x}}_{3}^{}-{{x}}_{4}^{}} \right) \left( \frac{{{x}}_{1}^{}-{{x}}_{4}^{}}{{{x}}_{2}^{}-{{x}}_{3}^{}} \right)  \\
\mathrm{Cross\ Product} & \frac{({{x}}_{1}^{}-{{x}}_{2}^{})({{x}}_{3}^{}-{{x}}_{4}^{})}{({{x}}_{1}^{}-{{x}}_{4}^{})({{x}}_{2}^{}-{{x}}_{3}^{})}  \\
\end{array}